Progress.v
@@ -1,0 +1,115 @@
+Require Import List.
+Require Import String.
+
+Require Import Lambda.
+Require Import TypeInv.
+Require Import CannonicalForm.
+
+Definition WellTyped (t : term) : Prop :=
+  exists r : type, Some r = typing t nil.
+
+Theorem Progress :
+  forall (t : term),
+    WellTyped t -> value t \/ exists t1 : term, eval t = Some t1.
+Proof.
+unfold WellTyped in |- *.
+induction t.
+ intro; left; simpl in |- *; tauto.
+
+ intro; left; simpl in |- *; tauto.
+
+ intro; left; simpl in |- *; tauto.
+
+ intro.
+ decompose [ex] H.
+ apply ApplyRel in H0.
+ decompose [ex] H0.
+ decompose [and] H1.
+ right.
+ generalize H2.
+ elim IHt1.
+  destruct t1.
+   simpl in |- *.
+   intros; discriminate.
+
+   simpl in |- *; intros; discriminate.
+
+   intros.
+   simpl in |- *.
+   case (eval t2).
+    intro.
+    exists (Apply (Lambda s t t1) t0).
+    reflexivity.
+
+    exists (subst t1 s t2).
+    reflexivity.
+
+   simpl in |- *.
+   intro; contradiction .
+
+   simpl in |- *; intro; contradiction .
+
+  simpl in |- *.
+  case (eval t1).
+   intros.
+   exists (Apply t t2).
+   reflexivity.
+
+   intro.
+   decompose [ex] H4.
+   discriminate.
+
+  exists (FunT x0 x).
+  exact H2.
+
+ intro.
+ right.
+ decompose [ex] H.
+ apply IfRel in H0.
+ inversion H0.
+ inversion H2.
+ simpl in |- *.
+ generalize H1.
+ destruct t1.
+  simpl in |- *; intro; discriminate.
+
+  intro; case b.
+   exists t2.
+   reflexivity.
+
+   exists t3; reflexivity.
+
+  simpl in |- *.
+  case (typing t1 ((s, t) :: nil)).
+   intro.
+   intro.
+   discriminate.
+
+   intro; discriminate.
+
+  elim IHt1.
+   simpl in |- *; intro; contradiction .
+
+   intro.
+   intro.
+   decompose [ex] H5.
+   rewrite H7 in |- *.
+   exists (If x0 t2 t3).
+   reflexivity.
+
+   rewrite <- H1 in |- *.
+   exists BoolT.
+   reflexivity.
+
+  elim IHt1.
+   simpl in |- *; intro; contradiction .
+
+   intros.
+   decompose [ex] H5.
+   rewrite H7 in |- *.
+   exists (If x0 t2 t3); reflexivity.
+
+   exists BoolT.
+   exact H1.
+Qed.
+
